Weidenbach_Book/WB_More_Refinement.thy
@@ -199,6 +199,24 @@ method match_spec_trans =
     \<open>print_term f; match premises in I: \<open>_ \<Longrightarrow> _ \<Longrightarrow> f' \<le> SPEC R'\<close> for f' :: \<open>'a nres\<close> and R' :: \<open>'a \<Rightarrow> bool\<close>
        \<Rightarrow> \<open>print_term f'; rule weaken_SPEC2[of f' R' f R]\<close>\<close>)
 
+subsection \<open>More Operations\<close>
+
+abbreviation "curry8' fc \<equiv> (\<lambda> (a, b, c, d, e, f, g, h). fc a b c d e f g)"
+
+abbreviation comp4 (infixl "oooo" 55) where "f oooo g \<equiv> \<lambda>x. f ooo (g x)"
+abbreviation comp5 (infixl "ooooo" 55) where "f ooooo g \<equiv> \<lambda>x. f oooo (g x)"
+abbreviation comp6 (infixl "oooooo" 55) where "f oooooo g \<equiv> \<lambda>x. f oooo (g x)"
+abbreviation comp7 (infixl "ooooooo" 55) where "f ooooooo g \<equiv> \<lambda>x. f oooo (g x)"
+abbreviation comp8 (infixl "oooooooo" 55) where "f oooooooo g \<equiv> \<lambda>x. f oooo (g x)"
+
+notation (in -)
+  comp4 (infixl "\<circ>\<circ>\<circ>" 55) and
+  comp5 (infixl "\<circ>\<circ>\<circ>\<circ>" 55) and
+  comp6 (infixl "\<circ>\<circ>\<circ>\<circ>\<circ>" 55) and
+  comp7 (infixl "\<circ>\<circ>\<circ>\<circ>\<circ>\<circ>" 55) and
+  comp8 (infixl "\<circ>\<circ>\<circ>\<circ>\<circ>\<circ>\<circ>" 55)
+
+
 subsection \<open>More Theorems for Refinement\<close>
 
 lemma bind_refine_spec: \<open>(\<And>x. \<Phi> x \<Longrightarrow> f x \<le> \<Down> R M) \<Longrightarrow> M' \<le> SPEC \<Phi> \<Longrightarrow> M' \<bind> f \<le> \<Down> R M\<close>
@@ -221,6 +239,10 @@ lemma hrp_comp_Id2[simp]: \<open>hrp_comp A Id = A\<close>
 
 
 subsection \<open>Some Refinement\<close>
+
+lemma (in -) fr_refl': \<open>A \<Longrightarrow>\<^sub>A B \<Longrightarrow> C * A \<Longrightarrow>\<^sub>A C * B\<close>
+  unfolding assn_times_comm[of C]
+  by (rule Automation.fr_refl)
 
 lemma Collect_eq_comp: \<open>{(c, a). a = f c} O {(x, y). P x y} = {(c, y). P (f c) y}\<close>
   by auto
